examples/crypto/cryptobox/Box.PlainDH.fst
@@ -28,3 +28,5 @@ let get_logGT = AE.get_logGT
 let recall_log = AE.recall_log
 
 let empty_log = AE.empty_log
+
+let nonce = AE.nonce
